Neighborhood/Logic/Logic/EMNK.lean
@@ -1,0 +1,50 @@
+module
+
+public import Neighborhood.Logic.Logic.EMN
+public import Neighborhood.Logic.Logic.EMK
+public import Neighborhood.Semantics.Example.Frame1_3
+public import Neighborhood.Semantics.Example.Frame2_138
+public import Neighborhood.Semantics.Example.Frame2_140
+
+@[expose] public section
+
+variable {α : Type u} {A : Formula α}
+
+namespace LogicEMNK
+
+theorem sound {κ} [Nonempty κ] (F : Frame κ) [F.IsMonotonic] [F.HasPropertyK]
+    [F.ContainsUnit] :
+    A ∈ LogicEMNK → F ⊧ A :=
+  Hilbert.sound (by rintro _ ((⟨_, _, rfl⟩ | rfl) | ⟨_, _, rfl⟩) <;> simp)
+
+instance : (@LogicEMNK α).IsConsistent := ⟨by
+  by_contra! hC
+  simpa using LogicEMNK.sound frame_1_2 hC⟩
+
+lemma not_provable_axiomT (a : α) : ∃ A, Axioms.T A ∉ (@LogicEMNK α) := by
+  by_contra! hcon
+  exact frame_1_3.not_valid_axiomT (LogicEMNK.sound frame_1_3 (hcon #a))
+
+lemma not_provable_axiomB (a : α) : ∃ A, Axioms.B A ∉ (@LogicEMNK α) := by
+  by_contra! hcon
+  exact frame_2_138.not_valid_axiomB (LogicEMNK.sound frame_2_138 (hcon #a))
+
+lemma not_provable_axiomD (a : α) : ∃ A, Axioms.D A ∉ (@LogicEMNK α) := by
+  by_contra! hcon
+  exact frame_1_3.not_valid_axiomD (LogicEMNK.sound frame_1_3 (hcon #a))
+
+lemma not_provable_axiomP : (Axioms.P : Formula α) ∉ (@LogicEMNK α) := by
+  intro hcon
+  exact frame_1_3.not_valid_axiomP (LogicEMNK.sound frame_1_3 hcon)
+
+lemma not_provable_axiomFour (a : α) : ∃ A, Axioms.Four A ∉ (@LogicEMNK α) := by
+  by_contra! hcon
+  exact frame_2_140.not_valid_axiomFour (LogicEMNK.sound frame_2_140 (hcon #a))
+
+lemma not_provable_axiomFive (a : α) : ∃ A, Axioms.Five A ∉ (@LogicEMNK α) := by
+  by_contra! hcon
+  exact frame_2_138.not_valid_axiomFive (LogicEMNK.sound frame_2_138 (hcon #a))
+
+end LogicEMNK
+
+end
